src/lib/wsat.v
@@ -5,27 +5,38 @@ From iris.base_logic.lib Require Export own.
 From iris.base_logic.lib Require Import wsat later_credits invariants.
 From iris.prelude Require Import options.
 
-From nextgen Require Import nextgen_pointwise.
+From nextgen Require Import nextgen_pointwise gmap_view_transformation.
   
 (** All definitions in this file are internal to [fancy_updates] with the
 exception of what's in the [wsatGS] module. The module [wsatGS] is thus exported in
 [fancy_updates], where [wsat] is only imported. *)
 Module wsatGS.
 
-Class wsatGIndpreS (Σ : gFunctors) (Ω : gTransformations Σ) : Set := WsatGIndpreS {
+Class pick_transform_preorder (A : cmra) : Type := TransPre {
+  C : Type;
+  CR : relation C;
+  C_pre :> PreOrder CR;
+  C_pick : C -> (A -> A);
+  C_pick_cmramorphism :> ∀ (c : C), CmraMorphism (C_pick c);
+  C_dec :> ∀ (c1 c2 : C), Decision (CR c1 c2)
+}.
+  
+Class wsatGIndpreS (Σ : gFunctors) (Ω : gTransformations Σ) (A : cmra) (pick: pick_transform_preorder A) : Set := WsatGIndpreS {
   wsatGpreS_inv : genIndInG Σ Ω (gmap_viewR positive (laterO (iPropO Σ)));
+  wsatGpreS_func : noTwoTransInG Σ Ω (gmap_viewR positive (optionO (leibnizO C))) A;
   wsatGpreS_enabled : genIndInG Σ Ω coPset_disjR;
   wsatGpreS_disabled : genIndInG Σ Ω (gset_disjR positive);
 }.
 
-Class wsatGIndS (Σ : gFunctors) (Ω : gTransformations Σ) : Set := WsatGInd {
-  wsat_inG : wsatGIndpreS Σ Ω;
+Class wsatGIndS (Σ : gFunctors) (Ω : gTransformations Σ) (A : cmra) (pick: pick_transform_preorder A) : Set := WsatGInd {
+  wsat_inG : wsatGIndpreS Σ Ω A pick;
   invariant_name : gname;
   enabled_name : gname;
   disabled_name : gname;
+  pick_name : gname;                                                                               
 }.
-Global Hint Mode wsatGIndpreS - - : typeclass_instances.
-Global Hint Mode wsatGIndS - - : typeclass_instances.
+Global Hint Mode wsatGIndpreS - - - - : typeclass_instances.
+Global Hint Mode wsatGIndS - - - - : typeclass_instances.
 
 
 Class lcGIndpreS (Σ : gFunctors) (Ω : gTransformations Σ) := LcGIndpreS {
@@ -44,12 +55,11 @@ Import wsatGS.
 Local Existing Instances wsat_inG wsatGpreS_inv wsatGpreS_enabled wsatGpreS_disabled.
 
 
-
-#[global] Instance into_wsatpres `{Hwsat: wsatGIndpreS Σ Ω} : wsatGpreS Σ :=
+#[global] Instance into_wsatpres `{pick: pick_transform_preorder A} `{!wsatGIndpreS Σ Ω A pick} : wsatGpreS Σ :=
   WsatGpreS Σ wsatGpreS_inv.(genInG_inG) wsatGpreS_enabled.(genInG_inG) wsatGpreS_disabled.(genInG_inG).
   
-#[global] Instance into_wsats `{Hwsat: wsatGIndS Σ Ω} : wsatGS Σ :=
-  WsatG Σ (@into_wsatpres Σ Ω wsat_inG) invariant_name enabled_name disabled_name.
+#[global] Instance into_wsats `{pick: pick_transform_preorder A} `{!wsatGIndS Σ Ω A pick} : wsatGS Σ  :=
+  WsatG Σ (@into_wsatpres A pick Σ Ω wsat_inG) invariant_name enabled_name disabled_name.
 
 #[global] Instance into_lcpres `{Hlc: lcGIndpreS Σ Ω} : lcGpreS Σ :=
   LcGpreS Σ lcGpreS_inG.(genInG_inG).
@@ -57,46 +67,118 @@ Local Existing Instances wsat_inG wsatGpreS_inv wsatGpreS_enabled wsatGpreS_disa
 #[global] Instance into_lcs `{Hlc: lcGIndS Σ Ω} : lcGS Σ :=
   LcGS Σ lcGS_inG.(genInG_inG) lcGS_name.
 
-Definition inv_cond `{!wsatGIndS Σ Ω} `{!noTransInG Σ Ω T} Q : iProp Σ := ■ (∀ (f : T → T) `{!CmraMorphism f}, Q -∗ ⚡={transmap_insert_inG f Ω}=> Q).
+#[global] Instance cmra_morphism_pick `{Hpre : pick_transform_preorder A} : ∀ c', CmraMorphism (C_pick c') :=
+  Hpre.(C_pick_cmramorphism).
 
-Definition wsat `{!wsatGIndS Σ Ω} `{!noTransInG Σ Ω T} : iProp Σ :=
-  locked (∃ I : gmap positive (iProp Σ),
-    own invariant_name (gmap_view_auth (DfracOwn 1) (invariant_unfold <$> I)) ∗
-    [∗ map] i ↦ Q ∈ I, inv_cond Q ∗ ((▷ Q ∗ ownD {[i]}) ∨ ownE {[i]}))%I.
+#[global] Instance wsat_notrans_inl `{wsat: !wsatGIndS Σ Ω A pick} : noTransInG Σ Ω A | 2 :=
+  (wsatGpreS_func.(noTransInG_B_inG)).
+
+#[global] Instance wsat_notrans_inr `{wsat: !wsatGIndS Σ Ω A pick} : noTransInG Σ Ω (gmap_viewR positive (optionO (leibnizO C))) | 2 :=
+  (wsatGpreS_func.(noTransInG_A_inG)).
+
+#[local] Instance inG_wsatGS_inl `{Hpre : wsatGIndpreS Σ Ω T} : inG Σ (gmap_viewR positive (optionO (leibnizO C))) :=
+  (wsatGpreS_func.(noTransInG_A_inG)).(noTransInG_inG).
+
+#[local] Instance inG_wsatGS_inr `{Hpre : wsatGIndpreS Σ Ω T} : inG Σ T :=
+  (wsatGpreS_func.(noTransInG_B_inG)).(noTransInG_inG).
+
+Definition pick_coerce `{pick_transform_preorder A} (c : option C) : optionO (leibnizO C) := c.
+
+Definition ownC `{pick: pick_transform_preorder A} `{!wsatGIndS Σ Ω A pick} (i : positive) (c : C) : iProp Σ :=
+  own pick_name (gmap_view_frag i DfracDiscarded (pick_coerce (Some c))).
+Global Typeclasses Opaque ownC.
+Global Instance: Params (@ownC) 2 := {}.
+
+Definition ownN `{pick: pick_transform_preorder A} `{!wsatGIndS Σ Ω A pick} (i : positive) : iProp Σ :=
+  own pick_name (gmap_view_frag i DfracDiscarded None).
+Global Typeclasses Opaque ownN.
+Global Instance: Params (@ownN) 1 := {}.
+
+#[global] Instance ownC_persistent `{pick: pick_transform_preorder A} `{!wsatGIndS Σ Ω A pick} (i : positive) (c : C) : Persistent (ownC i c).
+Proof. rewrite /ownC. apply _. Qed.
+#[global] Instance ownN_persistent `{pick: pick_transform_preorder A} `{!wsatGIndS Σ Ω A pick} (i : positive) : Persistent (ownN i).
+Proof. rewrite /ownN. apply _. Qed.
+
+
+Definition inv_pick_cut `{pick_transform_preorder A} (c : C) (i : positive) (v : optionO (leibnizO C)) :=
+ Some (v ≫= (λ c', if decide (CR c' c) then Some c' else None)).
+Definition inv_pick_transform `{pick_transform_preorder A} (c : C) := (map_entry_lift_gmap_view (inv_pick_cut c)).
+
+#[global] Instance inv_pick_mapTrans `{pick_transform_preorder A} (c : C) : MapTrans (inv_pick_cut c).
+Proof.
+  split.
+  - intros l v1 Hcontr. done.
+  - intros k n v1 v2 Hv1. rewrite /inv_pick_cut /=.
+    constructor. destruct v1,v2;inversion Hv1;simplify_eq =>/= //.
+    rewrite H2. auto.    
+Qed.
+
+#[global] Instance cmra_morphism_pick_transform `{pick_transform_preorder A} : ∀ c', CmraMorphism (inv_pick_transform c') :=
+  λ c', gMapTrans_lift_CmraMorphism (inv_pick_cut c').
+
+Definition inv_cond {Σ Ω A} `{pick: pick_transform_preorder A} {wsat: wsatGIndS Σ Ω A pick} Q (c : C) : iProp Σ :=
+  ■ (∀ (c' : C), ⌜CR c c'⌝ -∗ Q -∗ ⚡={transmap_insert_inG (inv_pick_transform c') Ω}=> ⚡={transmap_insert_inG (C_pick c') Ω}=> Q).
+
+Definition wsat `{pick: pick_transform_preorder A} `{!wsatGIndS Σ Ω A pick} : iProp Σ :=
+  locked (∃ (I : gmap positive (iProp Σ)) (F : gmap positive (option C)),
+    ⌜dom I = dom F⌝ ∗
+     own invariant_name (gmap_view_auth (DfracOwn 1) (invariant_unfold <$> I)) ∗
+     own pick_name (gmap_view_auth (DfracOwn 1) (pick_coerce <$> F)) ∗
+    [∗ map] i ↦ Q ∈ I, (ownN i ∨ ∃ (c : C), ownC i c ∗ inv_cond Q c ∗ (▷ Q ∗ ownD {[i]} ∨ ownE {[i]})))%I.
 
 Section wsat.
-Context `{!wsatGIndS Σ Ω} `{!noTransInG Σ Ω T}.
+Context `{!wsatGIndS Σ Ω A pick}.
 Implicit Types P : iProp Σ.
 
-Lemma ownI_open i P : wsat ∗ ownI i P ∗ ownE {[i]} ⊢ wsat ∗ ▷ P ∗ ownD {[i]}.
+Lemma ownCN i c : (ownC i c ∗ ownN i) ⊢ False.
 Proof.
-  rewrite /ownI /wsat -!lock.
-  iIntros "(Hw & Hi & HiE)". iDestruct "Hw" as (I) "[Hw HI]".
-  iDestruct (invariant_lookup I i P with "[$]") as (Q ?) "#HPQ".
-  iDestruct (big_sepM_delete _ _ i with "HI") as "[[#Hcond [[HQ $]|HiE']] HI]"; eauto.
-  - iSplitR "HQ"; last by iNext; iRewrite -"HPQ".
-    iExists I. iFrame "Hw". iApply (big_sepM_delete _ _ i); eauto.
-    iFrame "HI"; eauto.
-  - iDestruct (ownE_singleton_twice with "[$HiE $HiE']") as %[].
-Qed.
-Lemma ownI_close i P : wsat ∗ ownI i P ∗ ▷ P ∗ ownD {[i]} ⊢ wsat ∗ ownE {[i]}.
-Proof.
-  rewrite /ownI /wsat -!lock.
-  iIntros "(Hw & Hi & HP & HiD)". iDestruct "Hw" as (I) "[Hw HI]".
-  iDestruct (invariant_lookup with "[$]") as (Q ?) "#HPQ".
-  iDestruct (big_sepM_delete _ _ i with "HI") as "[[#?[[HQ ?]|$]] HI]"; eauto.
-  - iDestruct (ownD_singleton_twice with "[$]") as %[].
-  - iExists I. iFrame "Hw". iApply (big_sepM_delete _ _ i); eauto.
-    iFrame "HI #". iLeft. iFrame "HiD". by iNext; iRewrite "HPQ".
+  rewrite /ownC /ownN.
+  rewrite -own_op own_valid gmap_view_frag_op_validI option_equivI.
+  rewrite /pick_coerce. iIntros "[? ?]". done.
 Qed.
 
-Lemma ownI_alloc φ P :
+Lemma ownC_eq i c c' : (ownC i c ∗ ownC i c') ⊢ (⌜c = c'⌝).
+Proof.
+  rewrite /ownC /ownN.
+  rewrite -own_op own_valid gmap_view_frag_op_validI option_equivI.
+  rewrite /pick_coerce. iIntros "[? %]". iPureIntro. auto.
+Qed.
+
+Lemma ownI_open i c P : wsat ∗ ownI i P ∗ ownC i c ∗ ownE {[i]} ⊢ wsat ∗ ▷ P ∗ ownD {[i]}.
+Proof.
+  rewrite /ownI /wsat -!lock.
+  iIntros "(Hw & Hi & Hc & HiE)". iDestruct "Hw" as (I F Hdom) "[Hw [HF HI]]".
+  iDestruct (invariant_lookup I i P with "[$]") as (Q ?) "#HPQ".
+  iDestruct (big_sepM_delete _ _ i with "HI") as "[[Hnone|Hsome] HI]"; eauto.
+  - by iDestruct (ownCN with "[$]") as "?".
+  - iDestruct "Hsome" as (c') "[#Hc' [#Hcond [[HQ HD] | HiE']]]".
+    + iFrame. iSplitR "HQ"; last by iNext; iRewrite -"HPQ".
+      iExists I,F. iFrame "Hw HF". iSplit;auto. iApply (big_sepM_delete _ _ i); eauto.
+      iFrame "HI". iRight. eauto.
+    + iDestruct (ownE_singleton_twice with "[$HiE $HiE']") as %[].
+Qed.
+Lemma ownI_close i c P : wsat ∗ ownI i P ∗ ownC i c ∗ ▷ P ∗ ownD {[i]} ⊢ wsat ∗ ownE {[i]}.
+Proof.
+  rewrite /ownI /wsat -!lock.
+  iIntros "(Hw & Hi & Hc & HP & HiD)". iDestruct "Hw" as (I F Hdom) "[Hw [HF HI]]".
+  iDestruct (invariant_lookup with "[$]") as (Q ?) "#HPQ".
+  iDestruct (big_sepM_delete _ _ i with "HI") as "[[Hnone|Hsome] HI]"; eauto.
+  - by iDestruct (ownCN with "[$]") as "?".
+  - iDestruct "Hsome" as (c') "[#Hc' [#Hcond [[HQ HD] | HiE']]]".
+    + iDestruct (ownD_singleton_twice with "[$]") as %[].
+    + iFrame. iExists I, F. iFrame "Hw HF". iSplit;auto. iApply (big_sepM_delete _ _ i); eauto.
+      iFrame "HI #". iRight. iExists _.
+      iDestruct (ownC_eq with "[$]") as %Heq. subst c'.
+      iFrame "Hc' Hcond". iLeft. iFrame "HiD". by iNext; iRewrite "HPQ".
+Qed.
+
+Lemma ownI_alloc φ P c :
   (∀ E : gset positive, ∃ i, i ∉ E ∧ φ i) →
-  inv_cond P ∗
+  inv_cond P c ∗
   wsat ∗ ▷ P ==∗ ∃ i, ⌜φ i⌝ ∗ wsat ∗ ownI i P.
 Proof.
   iIntros (Hfresh) "[#Hcond [Hw HP]]". rewrite /wsat -!lock.
-  iDestruct "Hw" as (I) "[Hw HI]".
+  iDestruct "Hw" as (I F Hdom) "[Hw [HF HI]]".
   iMod (own_unit (gset_disjUR positive) disabled_name) as "HE".
   iMod (own_updateP with "[$]") as "HE".
   { apply (gset_disj_alloc_empty_updateP_strong' (λ i, I !! i = None ∧ φ i)).
@@ -106,18 +188,28 @@ Proof.
   iMod (own_update with "Hw") as "[Hw HiP]".
   { eapply (gmap_view_alloc _ i DfracDiscarded); last done.
     by rewrite /= lookup_fmap HIi. }
+  iMod (own_update with "HF") as "[HF HiC]".
+  { eapply (gmap_view_alloc _ i DfracDiscarded); last done.
+    rewrite /= lookup_fmap. assert (F !! i = None) as -> =>//.
+    apply not_elem_of_dom. rewrite -Hdom.
+    apply not_elem_of_dom =>//. }
   iModIntro; iExists i;  iSplit; [done|]. rewrite /ownI; iFrame "HiP".
-  iExists (<[i:=P]>I); iSplitL "Hw".
+  iExists (<[i:=P]>I),(<[i:=Some c]>F). iSplit.
+  { iPureIntro. set_solver. }
+  iSplitL "Hw".
+  { by rewrite fmap_insert. }
+  iSplitL "HF".
   { by rewrite fmap_insert. }
   iApply (big_sepM_insert _ I); first done.
-  iFrame "HI #". iLeft. by rewrite /ownD; iFrame.
+  iFrame "HI #". iRight. iExists c. rewrite /ownC. iFrame "HiC Hcond".
+  iLeft. by rewrite /ownD; iFrame.
 Qed.
 
-Lemma ownI_alloc_open φ P :
+Lemma ownI_alloc_open φ P c :
   (∀ E : gset positive, ∃ i, i ∉ E ∧ φ i) →
-  inv_cond P ∗ wsat ==∗ ∃ i, ⌜φ i⌝ ∗ (ownE {[i]} -∗ wsat) ∗ ownI i P ∗ ownD {[i]}.
+  inv_cond P c ∗ wsat ==∗ ∃ i, ⌜φ i⌝ ∗ (ownE {[i]} -∗ wsat) ∗ ownI i P ∗ ownD {[i]}.
 Proof.
-  iIntros (Hfresh) "[#Hcond Hw]". rewrite /wsat -!lock. iDestruct "Hw" as (I) "[Hw HI]".
+  iIntros (Hfresh) "[#Hcond Hw]". rewrite /wsat -!lock. iDestruct "Hw" as (I F Hdom) "[Hw [HF HI]]".
   iMod (own_unit (gset_disjUR positive) disabled_name) as "HD".
   iMod (own_updateP with "[$]") as "HD".
   { apply (gset_disj_alloc_empty_updateP_strong' (λ i, I !! i = None ∧ φ i)).
@@ -127,26 +219,37 @@ Proof.
   iMod (own_update with "Hw") as "[Hw HiP]".
   { eapply (gmap_view_alloc _ i DfracDiscarded); last done.
     by rewrite /= lookup_fmap HIi. }
+  iMod (own_update with "HF") as "[HF HiC]".
+  { eapply (gmap_view_alloc _ i DfracDiscarded); last done.
+    rewrite /= lookup_fmap. assert (F !! i = None) as -> =>//.
+    apply not_elem_of_dom. rewrite -Hdom.
+    apply not_elem_of_dom =>//. }
   iModIntro; iExists i;  iSplit; [done|]. rewrite /ownI; iFrame "HiP".
   unfold ownD. simpl. iFrame "HD".
-  iIntros "HE". iExists (<[i:=P]>I); iSplitL "Hw".
+  iIntros "HE". iExists (<[i:=P]>I),(<[i:=Some c]>F); iSplit.
+  { iPureIntro. set_solver. }
+  iSplitL "Hw".  
   { by rewrite fmap_insert. }
+  iSplitL "HF".  
+  { by rewrite fmap_insert. }  
   iApply (big_sepM_insert _ I); first done.
-  iFrame "HI #". by iRight.
+  iFrame "HI #". iRight. iExists _. rewrite /ownC. iFrame "HiC Hcond". by iRight.
 Qed.
 End wsat.
 
 (* Allocation of an initial world *)
-Lemma wsat_alloc `{!wsatGIndpreS Σ Ω} `{!noTransInG Σ Ω T} : ⊢ |==> ∃ _ : wsatGIndS Σ Ω, wsat ∗ ownE ⊤.
+Lemma wsat_alloc `{!wsatGIndpreS Σ Ω A pick} : ⊢ |==> ∃ _ : wsatGIndS Σ Ω A pick, wsat ∗ ownE ⊤.
 Proof.
   iIntros.
-  iMod (own_alloc (gmap_view_auth (DfracOwn 1) ∅)) as (γI) "HI";
+  iMod (own_alloc (@gmap_view_auth _ _ _ (laterO (iPropO Σ)) (DfracOwn 1) ∅)) as (γI) "HI";
+    first by apply gmap_view_auth_valid.
+  iMod (own_alloc (@gmap_view_auth _ _ _ (optionO (leibnizO C)) (DfracOwn 1) ∅)) as (γI') "HI'";
     first by apply gmap_view_auth_valid.
   iMod (own_alloc (CoPset ⊤)) as (γE) "HE"; first done.
   iMod (own_alloc (GSet ∅)) as (γD) "HD"; first done.
-  iModIntro; iExists (WsatGInd _ _ _ γI γE γD).
+  iModIntro. iExists (WsatGInd _ _ _ _ _ γI γE γD γI').
   rewrite /wsat /ownE -lock; iFrame.
-  iExists ∅. rewrite fmap_empty big_opM_empty. by iFrame.
+  iExists ∅,∅. rewrite fmap_empty big_opM_empty. by iFrame.
 Qed.
 
 Lemma lc_ind_insert_intro `{lcGIndS Σ Ω} `{noTransInG Σ Ω A} (m : nat) (t : A → A) `{!CmraMorphism t} :
@@ -157,13 +260,8 @@ Proof.
   iModIntro. iFrame.
 Qed.
 
-#[global]
-Instance lc_into_pnextgen `{lcGIndS Σ Ω} `{noTransInG Σ Ω A}
-    (m : nat) (t : A → A) `{!CmraMorphism t} : IntoPnextgen _ _ _ :=
-  lc_ind_insert_intro m t.
-
 Lemma lc_ind_intro `{lcGIndS Σ Ω} (m : nat) :
-  £ m -∗ ⚡={Ω}=> £ m.
+  £ m ⊢ ⚡={Ω}=> £ m.
 Proof.
   iIntros "Hm".
   unfold lc. rewrite seal_eq /= /later_credits.lc_def /=.
@@ -171,7 +269,7 @@ Proof.
 Qed.
 
 Lemma ls_ind_intro `{lcGIndS Σ Ω} (m : nat) :
-  later_credits.lc_supply m -∗ ⚡={Ω}=> later_credits.lc_supply m.
+  later_credits.lc_supply m ⊢ ⚡={Ω}=> later_credits.lc_supply m.
 Proof.
   iIntros "Hm".
   unfold later_credits.lc_supply. rewrite seal_eq /= /later_credits.lc_supply_def.
@@ -179,61 +277,260 @@ Proof.
 Qed.
 
 Lemma ls_ind_insert_intro `{lcGIndS Σ Ω} `{noTransInG Σ Ω A} (t : A → A) `{!CmraMorphism t} (m : nat) :
-  later_credits.lc_supply m -∗ ⚡={transmap_insert_inG t Ω}=> later_credits.lc_supply m.
+  later_credits.lc_supply m ⊢ ⚡={transmap_insert_inG t Ω}=> later_credits.lc_supply m.
 Proof.
   iIntros "Hm".
   unfold later_credits.lc_supply. rewrite seal_eq /= /later_credits.lc_supply_def.
   iModIntro. iFrame.
 Qed.
 
+Lemma ownE_ind_insert_intro `{!wsatGIndS Σ Ω A pick} `{noTransInG Σ Ω B} (E: coPset) (t : B → B) `{!CmraMorphism t} :
+  ownE E ⊢ ⚡={transmap_insert_inG t Ω}=> ownE E.
+Proof.
+  iIntros "Hwsat". rewrite /ownE.
+  iModIntro. iFrame.
+Qed.
 
-Lemma ownE_ind_insert_intro `{wsatGIndS Σ Ω} `{noTransInG Σ Ω A} (E: coPset) (t : A → A) `{!CmraMorphism t} :
-  ownE E -∗ ⚡={transmap_insert_inG t Ω}=> ownE E.
+Lemma ownE_ind_intro `{!wsatGIndS Σ Ω A pick} (E: coPset) :
+  ownE E ⊢ ⚡={Ω}=> ownE E.
 Proof.
   iIntros "Hwsat".
   unfold ownE.
   iModIntro. iFrame.
 Qed.
 
-Lemma ownE_ind_intro `{wsatGIndS Σ Ω} (E: coPset) :
-  ownE E -∗ ⚡={Ω}=> ownE E.
-Proof.
-  iIntros "Hwsat".
-  unfold ownE.
-  iModIntro. iFrame.
-Qed.
-
-Lemma ownD_ind_insert_intro `{wsatGIndS Σ Ω} `{noTransInG Σ Ω A} (E: gset positive) (t : A → A) `{!CmraMorphism t} :
-  ownD E -∗ ⚡={transmap_insert_inG t Ω}=> ownD E.
+Local Lemma ownD_ind_insert_intro' `{!wsatGIndS Σ Ω A pick} `{noTransInG Σ Ω B} (E: gset positive) (t : B → B) `{!CmraMorphism t} :
+  ownD E ⊢ ⚡={transmap_insert_inG t Ω}=> ownD E.
 Proof.
   iIntros "Hwsat".
   unfold ownD.
   iModIntro. iFrame.
+Qed.
+
+Lemma ownD_ind_insert_intro `{!wsatGIndS Σ Ω A pick} (E: gset positive) (c : C) : 
+  ownD E ⊢ ⚡={transmap_insert_inG (C_pick c) Ω}=> ownD E.
+Proof.
+  iIntros "Hwsat".
+  destruct wsatGIndS0,wsat_inG0.
+  assert (noTransInG Σ Ω A);[apply _|].
+  iApply (@ownD_ind_insert_intro' _ _ A _ _ A).
+  iFrame.
+Qed.
+
+Lemma ownD_ind_pick_map_intro `{!wsatGIndS Σ Ω A pick} (E: gset positive) (c : C) :
+  ownD E ⊢ ⚡={transmap_insert_inG (inv_pick_transform c) Ω}=> ownD E.
+Proof.
+  iIntros "Hwsat".
+  destruct wsatGIndS0,wsat_inG0.
+  assert (noTransInG Σ Ω A);[apply _|].
+  iApply ownD_ind_insert_intro'.
+  iFrame.
 Qed.
 
 Lemma ownD_ind_intro `{wsatGIndS Σ Ω} (E: gset positive) :
-  ownD E -∗ ⚡={Ω}=> ownD E.
+  ownD E ⊢ ⚡={Ω}=> ownD E.
 Proof.
   iIntros "Hwsat".
   unfold ownD.
   iModIntro. iFrame.
 Qed.
 
-Lemma wsat_ind_insert_intro `{wsatGIndS Σ Ω} `{noTransInG Σ Ω A} (t : A → A) `{!CmraMorphism t} :
-  wsat -∗ ⚡={transmap_insert_inG t Ω}=> wsat.
+Lemma auth_invariant_insert_intro `{!wsatGIndS Σ Ω A pick} `{i : noTransInG Σ Ω B} (I : gmap positive (laterO (iPropO Σ))) (t : B → B) `{!CmraMorphism t} :
+  own invariant_name (gmap_view_auth (DfracOwn 1) I)
+    ⊢ ⚡={transmap_insert_inG t Ω}=> own invariant_name (gmap_view_auth (DfracOwn 1) I).
+Proof.
+  iIntros "Hi".
+  iModIntro.
+  iFrame.
+Qed.
+
+Lemma auth_pick_map_insert_intro `{!wsatGIndS Σ Ω A pick} F (t : A → A) `{!CmraMorphism t}  :
+  own pick_name (gmap_view_auth (DfracOwn 1) F) ⊢
+    ⚡={transmap_insert_inG t Ω}=> own pick_name (gmap_view_auth (DfracOwn 1) F).
+Proof.
+  iIntros "Hc".
+  iApply transmap_own_insert_other_left. iFrame.
+Qed.
+
+Lemma auth_pick_map_transform_intro `{!wsatGIndS Σ Ω A pick} F (c : C) :
+  own pick_name (gmap_view_auth (DfracOwn 1) F) ⊢
+    ⚡={transmap_insert_inG (inv_pick_transform c) Ω}=> own pick_name (gmap_view_auth (DfracOwn 1) (map_imap (inv_pick_cut c) F)).
+Proof.
+  iIntros "Hc". rewrite -map_entry_lift_gmap_view_auth.
+  iApply transmap_own_insert. iFrame.
+Qed.
+
+Lemma frag_pick_map_insert_intro `{!wsatGIndS Σ Ω A pick} (i : positive) (c : C) (t : A → A) `{!CmraMorphism t} :
+  ownC i c ⊢
+    ⚡={transmap_insert_inG t Ω}=> ownC i c.
+Proof.
+  iIntros "Hc". rewrite /ownC.
+  iApply transmap_own_insert_other_left. iFrame.
+Qed.
+
+Lemma frag_pick_map_transform_Some_intro `{!wsatGIndS Σ Ω A pick} (i : positive) (c c' : C) :
+  CR c' c ->
+  ownC i c' ⊢
+    ⚡={transmap_insert_inG (inv_pick_transform c) Ω}=> ownC i c'.
+Proof.
+  iIntros (HCR) "Hc". rewrite /ownC.
+  iDestruct (@transmap_own_insert _ Σ Ω (@wsat_notrans_inr _ _ _ _ wsatGIndS0)
+               (inv_pick_transform c) with "Hc") as "Hc".
+  rewrite {2}/inv_pick_transform.
+  unfold map_entry_lift_gmap_view, cmra_morphism_extra.fmap_view, cmra_morphism_extra.fmap_pair. simpl.
+  rewrite /gMapTrans_frag_lift. rewrite -insert_empty.
+  erewrite map_imap_insert_Some;
+    [|rewrite /map_trans_frag_lift agree_option_map_to_agree /= //].
+  rewrite decide_True//.
+Qed.
+
+Lemma frag_pick_map_transform_None_intro `{!wsatGIndS Σ Ω A pick} (i : positive) (c c' : C) :
+  ¬ CR c' c ->
+  ownC i c' ⊢
+    ⚡={transmap_insert_inG (inv_pick_transform c) Ω}=> ownN i.
+Proof.
+  iIntros (HCR) "Hc". rewrite /ownC.
+  iDestruct (@transmap_own_insert _ Σ Ω (@wsat_notrans_inr _ _ _ _ wsatGIndS0)
+               (inv_pick_transform c) with "Hc") as "Hc".
+  rewrite {2}/inv_pick_transform.
+  unfold map_entry_lift_gmap_view, cmra_morphism_extra.fmap_view, cmra_morphism_extra.fmap_pair. simpl.
+  rewrite /gMapTrans_frag_lift. rewrite -insert_empty.
+  erewrite map_imap_insert_Some;
+    [|rewrite /map_trans_frag_lift agree_option_map_to_agree /= //].
+  rewrite decide_False//.
+Qed.
+
+Lemma frag_pick_map_None_intro `{!wsatGIndS Σ Ω A pick} (i : positive) (c : C) :
+  ownN i ⊢
+    ⚡={transmap_insert_inG (inv_pick_transform c) Ω}=> ownN i.
+Proof.
+  iIntros "Hc". rewrite /ownN.
+  iDestruct (@transmap_own_insert _ Σ Ω (@wsat_notrans_inr _ _ _ _ wsatGIndS0)
+               (inv_pick_transform c) with "Hc") as "Hc".
+  rewrite {2}/inv_pick_transform.
+  unfold map_entry_lift_gmap_view, cmra_morphism_extra.fmap_view, cmra_morphism_extra.fmap_pair. simpl.
+  rewrite /gMapTrans_frag_lift. rewrite -insert_empty.
+  erewrite map_imap_insert_Some;
+    [|rewrite /map_trans_frag_lift agree_option_map_to_agree /= //].
+  auto.
+Qed.
+
+Lemma ownN_insert_intro `{!wsatGIndS Σ Ω A pick} (i : positive) (t : A → A) `{!CmraMorphism t} :
+  ownN i ⊢ ⚡={transmap_insert_inG t Ω}=> ownN i.
+Proof.
+  iIntros "Hwsat".
+  rewrite /ownN.
+  iApply transmap_own_insert_other_left.
+  iFrame.
+Qed.
+
+Local Lemma transform_mono {Σ : gFunctors} {Ω : gTransformations Σ} (P : iProp Σ) :
+  (⚡={Ω}=> P) ⊢ ⚡={Ω}=> P.
+Proof.
+  apply nextgen_basic.bnextgen_mono.
+  iIntros "HP";done.
+Qed.
+
+Local Lemma transform_later {Σ : gFunctors} {Ω : gTransformations Σ} (P : iProp Σ) :
+  (▷ ⚡={Ω}=> P) ⊢ ⚡={Ω}=> ▷ P.
+Proof.
+  rewrite nextgen_basic.bnextgen_later.
+  auto.
+Qed.
+
+Local Lemma transform_plain {Σ : gFunctors} {Ω : gTransformations Σ} (P : iProp Σ) :
+  (■ P) ⊢ ⚡={Ω}=> ■ P.
+Proof.
+  iIntros "#HP".
+  iApply nextgen_basic.bnextgen_intro_plainly. eauto.
+Qed.
+
+#[local] Instance insert_mono_into_pnextgen {Σ : gFunctors} {Ω : gTransformations Σ} (P : iProp Σ)
+  : IntoPnextgen Ω _ _ := transform_mono P.
+#[local] Instance insert_later_into_pnextgen {Σ : gFunctors} {Ω : gTransformations Σ} (P : iProp Σ)
+  : IntoPnextgen Ω _ _ := transform_later P.
+#[local] Instance insert_plain_into_pnextgen {Σ : gFunctors} {Ω : gTransformations Σ} (P : iProp Σ)
+  : IntoPnextgen Ω _ _ := transform_plain P.
+
+Local Lemma map_imap_inv_pick_cut_coerce {A : cmra} `{pick: pick_transform_preorder A} (c : C) (F : gmap positive (option C)) :
+  pick_coerce <$> (map_imap (inv_pick_cut c) F) = map_imap (inv_pick_cut c) (pick_coerce <$> F).
+Proof.
+  induction F using map_ind.
+  - rewrite fmap_empty map_imap_empty //.
+  - rewrite fmap_insert !map_imap_insert.
+    destruct (inv_pick_cut c i x) eqn:Hc.
+    + rewrite fmap_insert.
+      assert (inv_pick_cut c i (pick_coerce x) = Some (pick_coerce o)) as ->;[|rewrite IHF//].
+      unfold inv_pick_cut.
+      unfold inv_pick_cut in Hc.
+      simpl. rewrite Hc. auto.
+    + done.
+Qed.
+
+Local Lemma dom_map_imap_inv_pick_cut {Σ} {A : cmra} `{pick: pick_transform_preorder A} (c : C) (I : gmap positive (iProp Σ)) (F : gmap positive (option C)) :
+  dom I = dom F ->
+  dom I = dom (map_imap (inv_pick_cut c) F).
+Proof.
+  intros Hdom.
+  rewrite (dom_imap_L _ _ (dom I))//.
+  intros i. split;intros Hi.
+  - rewrite Hdom in Hi.
+    apply elem_of_dom in Hi as [x Hx].
+    exists x. split;eauto.
+  - rewrite Hdom. apply elem_of_dom.
+    destruct Hi as [x [Hx Hsome]]. eauto.
+Qed.
+    
+Lemma wsat_ind_insert_intro `{!wsatGIndS Σ Ω A pick} (c : C) :
+  wsat -∗ ⚡={transmap_insert_inG (inv_pick_transform c) Ω}=> ⚡={transmap_insert_inG (C_pick c) Ω}=> wsat.
 Proof.
   iIntros "Hw". unfold wsat.
   rewrite -lock.
-  iDestruct "Hw" as (I) "[Hi H]".
-  iAssert ([∗ map] i↦Q ∈ I, ⚡={transmap_insert_inG t Ω}=> inv_cond Q ∗ (▷ Q ∗ ownD {[i]} ∨ ownE {[i]}))%I with "[H]" as "H".
+  iDestruct "Hw" as (I F Hdom) "[Hi [Hc H]]".
+  iAssert ([∗ map] i↦Q ∈ I, ⚡={transmap_insert_inG (inv_pick_transform c) Ω}=> ⚡={transmap_insert_inG (C_pick c) Ω}=>
+             ownN i ∨ (∃ c' : C, ownC i c' ∗ inv_cond Q c' ∗ (▷ Q ∗ ownD {[i]} ∨ ownE {[i]})))%I with "[H]" as "H".
   { iApply (big_sepM_mono with "H").
-    iIntros (k x Hx) "[#Hcond [[Hx Hi]|Hi]]".
-    - iAssert (▷ ⚡={transmap_insert_inG t Ω}=> x)%I with "[Hx]" as "Hx".
-      { iNext. by iApply "Hcond". }
-      iDestruct (ownD_ind_insert_intro with "Hi") as "Hi".
-      iModIntro. iFrame "#". iLeft. iFrame.
-    - iDestruct (ownE_ind_insert_intro with "Hi") as "Hi".
-      iModIntro. iFrame "#". iRight. iFrame. }
-  iDestruct (transmap_big_sepM_1 with "H") as "H".
-  iModIntro. iExists _. iFrame.
+    iIntros (k x Hx) "[HN | HC]".
+    - iDestruct (frag_pick_map_None_intro with "HN") as "HN".
+      iModIntro.
+      iDestruct (ownN_insert_intro _ (C_pick c) with "HN") as "HN".
+      iModIntro. iLeft. iFrame.
+    - iDestruct "HC" as (c') "[HC [#Hcond [[Hx HD] | HE]]]".
+      + destruct (decide (CR c' c)).
+        * iDestruct (frag_pick_map_transform_Some_intro with "HC") as "HC";[eauto|].
+          iAssert (▷ ⚡={transmap_insert_inG (inv_pick_transform c) Ω}=> ⚡={transmap_insert_inG (C_pick c) Ω}=> x)%I with "[Hx]" as "Hx".
+          { iNext. iApply ("Hcond" with "[//] [$]"). }
+          iDestruct (ownD_ind_pick_map_intro _ c with "HD") as "HD".
+          iModIntro.
+          iDestruct (frag_pick_map_insert_intro _ _ (C_pick c) with "HC") as "HC".
+          iDestruct (ownD_ind_insert_intro with "HD") as "HD".
+          iModIntro.
+          iRight. iExists c'. iFrame "Hcond HC". iLeft; iFrame.
+        * iDestruct (frag_pick_map_transform_None_intro with "HC") as "HC";[eauto|].
+          iClear "Hx Hcond HD". iModIntro.
+          iDestruct (ownN_insert_intro _ (C_pick c) with "HC") as "HC".
+          iModIntro. by iLeft.
+      + destruct (decide (CR c' c)).
+        * iDestruct (frag_pick_map_transform_Some_intro with "HC") as "HC";[eauto|].
+          iDestruct (ownE_ind_insert_intro  _ (inv_pick_transform c) with "HE") as "HE".
+          iModIntro.
+          iDestruct (frag_pick_map_insert_intro _ _ (C_pick c) with "HC") as "HC".
+          iDestruct (ownE_ind_insert_intro  _ (C_pick c) with "HE") as "HE".
+          iModIntro.
+          iRight. iExists c'. iFrame "Hcond HC". iRight. iFrame.
+        * iDestruct (frag_pick_map_transform_None_intro with "HC") as "HC";[eauto|].
+          iClear "HE Hcond". iModIntro.
+          iDestruct (ownN_insert_intro _ (C_pick c) with "HC") as "HC".
+          iModIntro. by iLeft. }
+  rewrite transmap_big_sepM_1.
+  iDestruct (auth_pick_map_transform_intro _ c with "Hc") as "Hc".
+  iDestruct (auth_invariant_insert_intro _ (inv_pick_transform c) with "Hi") as "Hi".
+  iModIntro.
+  rewrite transmap_big_sepM_1.
+  iDestruct (auth_pick_map_insert_intro _ (C_pick c) with "Hc") as "Hc".
+  iDestruct (auth_invariant_insert_intro _ (C_pick c) with "Hi") as "Hi".
+  iModIntro. iExists I,(map_imap (inv_pick_cut c) F). iFrame.
+  rewrite map_imap_inv_pick_cut_coerce. iFrame.
+  iPureIntro.
+  apply dom_map_imap_inv_pick_cut=>//.
 Qed.
